Prove Corollaries 1 and 2

ldqe.lean
@@ -17,7 +17,7 @@ def lift_eq_qe (β : Type) [atomeq α β] (qe : list α → fm α) (as : list α
     list_conj  (list.map (λ (a : α), A' (subst0 β eq a)) rest)
   end
 
-lemma ldqe_prsv [atomeq α β] (qe : list α → fm α) 
+lemma leq_is_dnf_qe [atomeq α β] (qe : list α → fm α) 
   (H : ∀ (as : list α), (∀ (a : α), a ∈ as → atom.dep0 β a ∧ ¬ solv0 β a) → is_dnf_qe β qe as) : 
   ∀ (as : list α), (∀ (a : α), a ∈ as → atom.dep0 β a) → is_dnf_qe β (lift_eq_qe β qe) as := 
 begin
@@ -79,172 +79,35 @@ begin
   apply mem_of_mem_filter H5, apply or.inl, refl
 end
 
-#check @nth_dft_pred
+def lift_dnfeq_qe (β : Type) [atomeq α β] (qe : list α → fm α) := lift_dnf_qe β (@lift_eq_qe α β _ qe) 
 
-#exit 
-  of_mem_of_mem :
-  ∀ {as : list α} {bs : list β} {a : α} {b : β}, 
-    a ∈ as → b ∈ bs → (a,b) ∈ list.product as bs 
-| [] _ _ _ H _ := by cases H
-| _ [] _ _ _ H := by cases H
-| (a::as) (b::bs) a' b' Ha Hb := 
-  begin
-    unfold has_mem.mem at Ha, unfold list.mem at Ha, 
-    unfold has_mem.mem at Hb, unfold list.mem at Hb, 
-    unfold has_mem.mem, unfold list.product, unfold list.map, 
-    unfold append, simp, unfold list.mem,
-    cases Ha with Ha Ha, cases Hb with Hb Hb, 
-    apply or.inl, simp *, 
-    apply or.inr, apply mem_append_of_mem_or_mem,
-    apply or.inl, simp *, apply mem_map_of_mem bs b', 
-    apply Hb, apply or.inr, apply mem_append_of_mem_or_mem,
-    apply or.inr, apply mem_product_of_mem_of_mem,
-    apply Ha, apply Hb
-  end
-
-lemma map_dist_append {f : α → β} : 
-  ∀ (l1 l2 : list α), list.map f (l1 ++ l2) = (list.map f l1) ++ (list.map f l2) := 
+lemma leq_qfree [HA : atomeq α β] (qe : list α → fm α)
+(Hqe : ∀ (as' : list α), allp (atom.dep0 β) as' → qfree (qe as'))
+(l : list α) (Hl : allp (atom.dep0 β) l) : qfree (lift_eq_qe β qe l) := 
 begin
-  intro l1, induction l1, intro l2, simp *,
-  intro l2, rename a_1 l1,
-  repeat {unfold append, unfold list.append}, 
-  repeat {unfold list.map}, unfold list.append,
-  apply congr_arg (list.cons (f a)), apply ih_1
+  unfold lift_eq_qe, simp,
+  cases (list.first (solv0 β) _) with pr,
+  apply Hqe, intros x Hx, apply Hl,
+  apply mem_of_mem_filter Hx, cases pr with eqn as',
+  apply list_conj_qfree, intros a Ha, 
+  cases (exp_mem_map Ha) with a' Ha',
+  rewrite Ha'^.elim_right, simp 
 end
 
-def mem_filter_of_pred_and_mem {P : α → Prop} [HD : decidable_pred P] : ∀ (as : list α) (a : α), P a → a ∈ as → a ∈ list.filter P as 
-| [] a HP HM := by cases HM 
-| (a'::as) a HP HM := 
-  begin
-    unfold list.filter, unfold ite, 
-    unfold has_mem.mem at HM, unfold list.mem at HM,
-    cases HM with HM HM, 
-    cases (HD a') with HD HD, 
-    exfalso, apply HD, rewrite HM at HP, apply HP,
-    simp, apply or.inl HM,  
-    cases (HD a') with HD HD, simp, 
-    apply mem_filter_of_pred_and_mem, apply HP, 
-    apply HM, simp, 
-    apply or.inr, apply mem_filter_of_pred_and_mem,
-    apply HP, apply HM
-  end
-
-lemma map_compose (f : α → β) (g : β → γ) : ∀ (as : list α), list.map g (list.map f as) = list.map (λ x, g (f x)) as 
-| [] :=eq.refl _
-| (a::as) := by simp 
-
-lemma exp_compose (f : α → β) (g : β → γ) (a : α) : (λ x, g (f x)) a = g (f a) := eq.refl _ 
-
-lemma map_eq (f g : α → β)  : ∀ (as : list α) (H : ∀ a, a ∈ as → f a = g a), list.map f as = list.map g as 
-| [] _ := eq.refl _
-| (a::as) H := 
-  begin 
-    unfold list.map, rewrite H, rewrite map_eq,
-    intros a Ha, apply (H _ (or.inr Ha)),  
-    apply (or.inl (eq.refl _))
-  end
-
-def dec_not_pred_of_dec_pred (P : α → Prop) [H : decidable_pred P] : decidable_pred (λ x, ¬ P x) := 
+lemma ldeq_prsv [atomeq α β] (qe : list α → fm α) (as : list α) 
+  (Hqe : ∀ (as') (Has' : allp (@atom.dep0 α β _) as'), qfree (qe as')) 
+  (Has : ∀ (as' : list α), (∀ (a' : α), a' ∈ as' → atom.dep0 β a' ∧ ¬ solv0 β a') → is_dnf_qe β qe as')  
+  (p : fm α) (bs : list β) : I (lift_dnfeq_qe β qe p) bs = I p bs := 
 begin
-  intro a, cases (H a) with H H, 
-  apply decidable.is_true H, 
-  apply decidable.is_false (not_not_intro H)
+  unfold lift_dnfeq_qe, apply ldq_prsv, apply leq_qfree,
+  apply Hqe, apply leq_is_dnf_qe, apply Has
 end
 
-open tactic
-
-meta def papply pe := to_expr pe >>= apply  
-
-meta def intro_fresh : tactic expr :=
-get_unused_name `h none >>= tactic.intro 
-
-meta def intro_refl : tactic unit := 
-do t ← target, 
-   match t with 
-   | `(_ = _) := papply ``(eq.refl _)
-   | `(_ → _) := intro_fresh >> intro_refl
-   | _ := failed 
-   end
-
-lemma iff_not_not {p : Prop} : p ↔ ¬¬p := 
-iff.intro (not_not_intro) (classical.by_contradiction)
-
-lemma iff_not_and {p q : Prop} : ¬ p ∨ ¬ q ↔ ¬(p ∧ q) := 
-iff.intro 
- (λ H1 H2, or.elim H1 (λ H3, H3 H2^.elim_left) (λ H3, H3 H2^.elim_right)) 
- (λ H, @classical.by_cases p _ 
-   (λ Hp, @classical.by_cases q _ 
-     (λ Hq, @false.rec _ (H $ and.intro Hp Hq)) 
-     (λ Hq, or.inr Hq))
-   (λ Hp, or.inl Hp))
-
-lemma iff_not_or {p q : Prop} : ¬ p ∧ ¬ q ↔ ¬(p ∨ q) :=  
-iff.intro 
-  (λ H, not_or H^.elim_left H^.elim_right)
-  (λ H, and.intro (λ Hp, H $ or.inl Hp) (λ Hq, H $ or.inr Hq)) 
-
-meta def first_arg (f : α → tactic β) : list α → tactic β 
-| [] := failed 
-| (a::as) := f a <|> (first_arg as)
-
-meta def papply_trans (pe : pexpr) := 
-do papply ``(eq.trans), papply pe
-
-
-lemma allp_filter (P : α → Prop) [H : decidable_pred P] : ∀ (l : list α) , allp P (list.filter P l) 
-| [] := begin intros _ Ha, cases Ha end 
-| (x::xs) := 
-  begin 
-    unfold list.filter, unfold ite, 
-    cases (H x) with H1 H1, simp, apply allp_filter, 
-    simp, intros a Ha, cases Ha with H2 H3, rewrite H2,
-    apply H1, apply allp_filter, apply H3
-  end
-
-lemma mem_of_mem_filter {P : α → Prop} {a : α} : 
-  ∀ {l : list α} {HD : decidable_pred P}, a ∈ (@list.filter _ P HD l) → a ∈ l  
-| [] _ := by {intro H, cases H} 
-| (a'::as) HD := 
-  begin
-    unfold list.filter, unfold ite, 
-    cases (HD a') with HD HD, simp, intro HM, 
-    apply or.inr, apply mem_of_mem_filter HM,
-    simp, intro HM, cases HM with H1 H2, 
-    apply or.inl H1, apply or.inr, 
-    apply mem_of_mem_filter H2,
-  end 
-
-lemma pred_of_mem_filter_pred {P : α → Prop} {a : α} : 
-  ∀ {l : list α} {HD : decidable_pred P}, a ∈ (@list.filter _ P HD l) → P a 
-| [] HD := by {intro H, cases H} 
-| (a'::as) HD := 
-  begin
-    unfold list.filter, unfold ite, 
-    cases (HD a') with HD HD, simp, 
-    intro Ha, apply pred_of_mem_filter_pred, apply Ha,
-    intro Ha, cases Ha with Ha Ha, rewrite Ha, apply HD,
-    apply pred_of_mem_filter_pred, apply Ha
-  end 
-
-lemma ex_iff_ex (P Q : α → Prop) (H : ∀ a, P a ↔ Q a) : (∃ x, P x) ↔ (∃ x, Q x) :=
+lemma ldeq_qfree [atomeq α β] (qe : list α → fm α) 
+  (Hqe : ∀ (as') (Has' : allp (@atom.dep0 α β _) as'), qfree (qe as')) 
+  (p : fm α) : qfree (lift_dnfeq_qe β qe p) := 
 begin
-  apply iff.intro, intro HP, cases HP with a Ha,
-  existsi a, apply (H a)^.elim_left Ha, 
-  intro HQ, cases HQ with a Ha,
-  existsi a, apply (H a)^.elim_right Ha 
-end
-
-lemma ex_eq_ex (P Q : α → Prop) (H : ∀ a, P a = Q a) : (∃ x, P x) = (∃ x, Q x) :=
-begin
-  apply propext, apply iff.intro, 
-  intro HP, cases HP with a Ha,
-  existsi a, rewrite H at Ha, apply Ha,
-  intro HQ, cases HQ with a Ha,
-  existsi a, rewrite H, apply Ha
-end
-
-lemma ex_to_ex (P Q : α → Prop) (H : ∀ a, P a → Q a) : (∃ x, P x) → (∃ x, Q x) := 
-begin
-  intro HP, cases HP with x Hx, 
-  existsi x, apply (H x Hx)
+  unfold lift_dnfeq_qe, apply ldq_qfree, 
+  intros as Has, apply leq_qfree, apply Hqe,
+  apply Has
 end
